Brought back the wallet example

examples/rel/IfcDelimitedRelease.fst
@@ -54,121 +54,121 @@ val verify_test (x y z: ref int):
 let verify_test x y z = ()
 
 
-(* val sum : prog 6 *)
-(* let sum [x1;x2;x3;x4;x5;y] h = *)
-(*   upd h y ((sel h x1 + sel h x2 + sel h x3 + sel h x4 + sel h x5)) *)
+val sum : prog 6
+let sum [x1;x2;x3;x4;x5;y] h =
+  upd h y ((sel h x1 + sel h x2 + sel h x3 + sel h x4 + sel h x5))
 
-(* val verify_sum (x1 x2 x3 x4 x5 y : ref int): *)
-(*   Lemma *)
-(*     (del_rel 6 *)
-(*       (fun r -> *)
-(*         if r = y then Low *)
-(*         else if List.Tot.mem r [x1;x2;x3;x4;x5] then High *)
-(*         else Low) *)
-(*       [x1;x2;x3;x4;x5;y] *)
-(*       [fun h -> sel h x1 + sel h x2 + sel h x3 + sel h x4 + sel h x5] *)
-(*       [] *)
-(*       sum) *)
-(* let verify_sum x1 x2 x3 x4 x5 y = () *)
+val verify_sum (x1 x2 x3 x4 x5 y : ref int):
+  Lemma
+    (del_rel 6
+      (fun r ->
+        if r = y then Low
+        else if List.Tot.mem r [x1;x2;x3;x4;x5] then High
+        else Low)
+      [x1;x2;x3;x4;x5;y]
+      [fun h -> sel h x1 + sel h x2 + sel h x3 + sel h x4 + sel h x5]
+      []
+      sum)
+let verify_sum x1 x2 x3 x4 x5 y = ()
 
-(* val sum_swap : prog 6 *)
-(* let sum_swap [x1;x2;x3;x4;x5;y] h = *)
-(*   let tmp1 = sel h x1 in *)
-(*   let h = upd h x1 (sel h x2) in *)
-(*   let h = upd h x2 (sel h x3) in *)
-(*   let h = upd h x3 (sel h x4) in *)
-(*   let h = upd h x4 (sel h x5) in *)
-(*   let h = upd h x5 tmp1 in *)
-(*   upd h y ((sel h x1 + sel h x2 + sel h x3 + sel h x4 + sel h x5)) *)
+val sum_swap : prog 6
+let sum_swap [x1;x2;x3;x4;x5;y] h =
+  let tmp1 = sel h x1 in
+  let h = upd h x1 (sel h x2) in
+  let h = upd h x2 (sel h x3) in
+  let h = upd h x3 (sel h x4) in
+  let h = upd h x4 (sel h x5) in
+  let h = upd h x5 tmp1 in
+  upd h y ((sel h x1 + sel h x2 + sel h x3 + sel h x4 + sel h x5))
 
-(* val verify_sum_swap (x1 x2 x3 x4 x5 y : ref int): *)
-(*   Lemma *)
-(*     (del_rel 6 *)
-(*       (fun r -> *)
-(*         if r = y then Low *)
-(*         else if List.Tot.mem r [x1;x2;x3;x4;x5] then High *)
-(*         else Low) *)
-(*       [x1;x2;x3;x4;x5;y] *)
-(*       [fun h -> sel h x1 + sel h x2 + sel h x3 + sel h x4 + sel h x5] *)
-(*       [] *)
-(*       sum_swap) *)
-(* let verify_sum_swap x1 x2 x3 x4 x5 y = () *)
+val verify_sum_swap (x1 x2 x3 x4 x5 y : ref int):
+  Lemma
+    (del_rel 6
+      (fun r ->
+        if r = y then Low
+        else if List.Tot.mem r [x1;x2;x3;x4;x5] then High
+        else Low)
+      [x1;x2;x3;x4;x5;y]
+      [fun h -> sel h x1 + sel h x2 + sel h x3 + sel h x4 + sel h x5]
+      []
+      sum_swap)
+let verify_sum_swap x1 x2 x3 x4 x5 y = ()
 
-(* val sum_att : prog 6 *)
-(* let sum_att [x1;x2;x3;x4;x5;y] h = *)
-(*   let tmp1 = sel h x1 in *)
-(*   let h = upd h x2 tmp1 in *)
-(*   let h = upd h x3 tmp1 in *)
-(*   let h = upd h x4 tmp1 in *)
-(*   let h = upd h x5 tmp1 in *)
-(*   upd h y ((sel h x1 + sel h x2 + sel h x3 + sel h x4 + sel h x5)) *)
+val sum_att : prog 6
+let sum_att [x1;x2;x3;x4;x5;y] h =
+  let tmp1 = sel h x1 in
+  let h = upd h x2 tmp1 in
+  let h = upd h x3 tmp1 in
+  let h = upd h x4 tmp1 in
+  let h = upd h x5 tmp1 in
+  upd h y ((sel h x1 + sel h x2 + sel h x3 + sel h x4 + sel h x5))
 
-(* (\* This does not verify, as expected *\) *)
-(* (\* *)
-(* val verify_sum_att (x1 x2 x3 x4 x5 y : ref int): *)
-(*   Lemma *)
-(*     (del_rel 6 *)
-(*       (fun r -> *)
-(*         if r = y then Low *)
-(*         else if List.Tot.mem r [x1;x2;x3;x4;x5] then High *)
-(*         else Low) *)
-(*       [x1;x2;x3;x4;x5;y] *)
-(*       [fun h -> sel h x1 + sel h x2 + sel h x3 + sel h x4 + sel h x5] *)
-(*       sum_att) *)
-(* let verify_sum_att x1 x2 x3 x4 x5 y = () *)
-(* *\) *)
+(* This does not verify, as expected *)
+(*
+val verify_sum_att (x1 x2 x3 x4 x5 y : ref int):
+  Lemma
+    (del_rel 6
+      (fun r ->
+        if r = y then Low
+        else if List.Tot.mem r [x1;x2;x3;x4;x5] then High
+        else Low)
+      [x1;x2;x3;x4;x5;y]
+      [fun h -> sel h x1 + sel h x2 + sel h x3 + sel h x4 + sel h x5]
+      sum_att)
+let verify_sum_att x1 x2 x3 x4 x5 y = ()
+*)
 
 
-(* val wallet : prog 3 *)
-(* let wallet [x_h;k;x_l] h = *)
-(*   if (sel h x_h >= sel h k) then *)
-(*     let h = upd h x_h (sel h x_h - sel h k) in *)
-(*     let h = upd h x_l (sel h x_l + sel h k) in *)
-(*     h *)
-(*   else *)
-(*     h *)
+val wallet : prog 3
+let wallet [x_h;k;x_l] h =
+  if (sel h x_h >= sel h k) then
+    let h = upd h x_h (sel h x_h - sel h k) in
+    let h = upd h x_l (sel h x_l + sel h k) in
+    h
+  else
+    h
 
-(* val verify_wallet (x_h k x_l : ref int): *)
-(*   Lemma *)
-(*     (del_rel 3 *)
-(*       (fun r -> *)
-(*         if r = x_h then High *)
-(*         else Low) *)
-(*       [x_h; k; x_l] *)
-(*       [] *)
-(*       [fun h -> sel h x_h >= sel h k] *)
-(*       wallet) *)
-(* let verify_wallet x_h k x_l = () *)
+val verify_wallet (x_h k x_l : ref int):
+  Lemma
+    (del_rel 3
+      (fun r ->
+        if r = x_h then High
+        else Low)
+      [x_h; k; x_l]
+      []
+      [fun h -> sel h x_h >= sel h k]
+      wallet)
+let verify_wallet x_h k x_l = ()
 
-(* // This is not accepted *)
-(* //val wallet_attack_loop : prog 4 *)
-(* val wallet_attack_loop : vl:list(ref int){List.Tot.length vl = 4 /\ List.Tot.noRepeats vl} -> h:heap -> GTot heap (decreases (sel h (List.Tot.hd vl))) *)
-(* let rec wallet_attack_loop [n;x_h;k;x_l] h = *)
-(*   if sel h n <= 0 then *)
-(*     h *)
-(*   else *)
-(*     let h = upd h k (pow2 (sel h n - 1)) in *)
-(*     let h = wallet [x_h;k;x_l] h in *)
-(*     let h = upd h n (sel h n - 1) in *)
-(*     wallet_attack_loop [n;x_h;k;x_l] h *)
+// This is not accepted
+//val wallet_attack_loop : prog 4
+val wallet_attack_loop : vl:list(ref int){List.Tot.length vl = 4 /\ List.Tot.noRepeats vl} -> h:heap -> GTot heap (decreases (sel h (List.Tot.hd vl)))
+let rec wallet_attack_loop [n;x_h;k;x_l] h =
+  if sel h n <= 0 then
+    h
+  else
+    let h = upd h k (pow2 (sel h n - 1)) in
+    let h = wallet [x_h;k;x_l] h in
+    let h = upd h n (sel h n - 1) in
+    wallet_attack_loop [n;x_h;k;x_l] h
 
-(* val wallet_attack : prog 4 *)
-(* let wallet_attack [n;x_h;k;x_l] h = *)
-(*  let h = upd h x_l 0 in *)
-(*  wallet_attack_loop [n;x_h;k;x_l] h *)
+val wallet_attack : prog 4
+let wallet_attack [n;x_h;k;x_l] h =
+ let h = upd h x_l 0 in
+ wallet_attack_loop [n;x_h;k;x_l] h
 
-(* (\* This does not verify, as expected *)
-(*    Howver, also does not verify wieht x_h : Low, which should be fine *\) *)
-(* (\* *)
-(* val verify_wallet_attack (n x_h k x_l : ref int): *)
-(*   Lemma *)
-(*     (del_rel 4 *)
-(*       (fun r -> *)
-(*         if r = x_h then High *)
-(*         else Low) *)
-(*       [n; x_h; k; x_l] *)
-(*       [] *)
-(*       [fun h -> sel h x_h >= sel h k] *)
-(*       wallet_attack) *)
-(* let verify_wallet_attack n x_h k x_l = () *)
-(* *\) *)
+(* This does not verify, as expected
+   Howver, also does not verify wieht x_h : Low, which should be fine *)
+(*
+val verify_wallet_attack (n x_h k x_l : ref int):
+  Lemma
+    (del_rel 4
+      (fun r ->
+        if r = x_h then High
+        else Low)
+      [n; x_h; k; x_l]
+      []
+      [fun h -> sel h x_h >= sel h k]
+      wallet_attack)
+let verify_wallet_attack n x_h k x_l = ()
+*)
